\documentclass{article}
\usepackage{amsmath}

\begin{document}
  \begin{equation}
    \frac{\partial J}{\partial z^l} = \delta^l
  \end{equation}
  \begin{equation}
    \frac{\partial J}{\partial \Delta^l} = (W^{l + 1})^T \delta^{l + 1} = \frac{\partial J}{\partial a^l}
  \end{equation}
  \begin{equation}
    \frac{\partial a^l}{\partial z^l} = \sigma(z^l) \odot (1 - \sigma(z^l))
  \end{equation}
  \begin{equation}
    \frac{\partial J}{\partial z^l} = \frac{\partial J}{\partial a^l} \frac{\partial a^l}{\partial z^l} = (W^{l + 1})^T \delta^{l + 1} \odot \sigma(z^l) \odot (1 - \sigma(z^l)) = \delta^l
  \end{equation}
\end{document}
